---
marp: true
theme: dracula
---

<!-- _class: slide__title -->

# The SAT, fast and slow

---

<!-- _class: slide__part -->

## Part 1: Theory.

---

<!-- _class: slide__chapter -->

### Sum of solutions

---

<!-- _class: slide__section -->

#### The General Form

---

<!-- _class: slide__section__subtitle -->

##### Example 1

---

<!-- _class: slide__algebra -->

$$x^2 = 16$$

---

<!-- _class: slide__algebra -->

$$x^2 = 16$$

$$x = \pm 4$$

---

<!-- _class: slide__algebra -->

$$x^2 = 16$$

$$x = \pm 4$$

$$x_1 \cdot x_2 = -4 \cdot 4 = -16$$

---

<!-- _class: slide__chapter -->

### Product of solutions

---

<!-- _class: slide__section -->

#### The vertex form

---

<!-- _class: slide__section__subtitle -->

##### Generalizing

---

<!-- _class: slide__algebra -->

$$x = \frac{-b}{2a} \pm \frac{\sqrt{b^2 - 4ac}}{2a}$$

---

<!-- _class: slide__algebra -->

$$x = \frac{-b}{2a} \pm \frac{\sqrt{b^2 - 4ac}}{2a}$$

$$x_1 \cdot x_2 = \left( -\frac{b}{2a} - \frac{\sqrt{b^2 - 4ac}}{2a} \right) \left( -\frac{b}{2a} + \frac{\sqrt{b^2 - 4ac}}{2a} \right)$$

---

<!-- _class: slide__algebra -->

$$x = \frac{-b}{2a} \pm \frac{\sqrt{b^2 - 4ac}}{2a}$$

$$x_1 \cdot x_2 = \left( -\frac{b}{2a} - \frac{\sqrt{b^2 - 4ac}}{2a} \right) \left( -\frac{b}{2a} + \frac{\sqrt{b^2 - 4ac}}{2a} \right)$$

$$x_1 \cdot x_2 = \left( -\frac{b}{2a} \right)^2 - \left( \frac{\sqrt{b^2 - 4ac}}{2a} \right)^2$$

---

<!-- _class: slide__algebra -->

$$x = \frac{-b}{2a} \pm \frac{\sqrt{b^2 - 4ac}}{2a}$$

$$x_1 \cdot x_2 = \left( -\frac{b}{2a} - \frac{\sqrt{b^2 - 4ac}}{2a} \right) \left( -\frac{b}{2a} + \frac{\sqrt{b^2 - 4ac}}{2a} \right)$$

$$x_1 \cdot x_2 = \left( -\frac{b}{2a} \right)^2 - \left( \frac{\sqrt{b^2 - 4ac}}{2a} \right)^2$$

$$x_1 \cdot x_2 = \frac{b^2}{(2a)^2} - \frac{b^2 - 4ac}{(2a)^2}$$

---

<!-- _class: slide__algebra -->

$$x_1 \cdot x_2 = \frac{b^2}{(2a)^2} - \frac{b^2 - 4ac}{(2a)^2}$$

---

<!-- _class: slide__algebra -->

$$x_1 \cdot x_2 = \frac{b^2}{(2a)^2} - \frac{b^2 - 4ac}{(2a)^2}$$

$$x_1 \cdot x_2 = \frac{b^2 - (b^2 - 4ac)}{4a^2}$$

---

<!-- _class: slide__algebra -->

$$x_1 \cdot x_2 = \frac{b^2}{(2a)^2} - \frac{b^2 - 4ac}{(2a)^2}$$

$$x_1 \cdot x_2 = \frac{b^2 - (b^2 - 4ac)}{4a^2}$$

$$x_1 \cdot x_2 = \frac{4ac}{4a^2}$$

---

<!-- _class: slide__algebra -->

$$x_1 \cdot x_2 = \frac{b^2}{(2a)^2} - \frac{b^2 - 4ac}{(2a)^2}$$

$$x_1 \cdot x_2 = \frac{b^2 - (b^2 - 4ac)}{4a^2}$$

$$x_1 \cdot x_2 = \frac{4ac}{4a^2}$$

$$x_1 \cdot x_2 = \frac{c}{a}$$

---
